compiler/InterpreterStatements.ml
@@ -811,12 +811,12 @@ let rec eval_statement (config : C.config) (st : A.statement) : st_cm_fun =
                   let expr = assign_to_place config rv p (cf Unit) ctx in
                   (* Update the synthesized AST - here we store meta-information.
                    * We do it only in specific cases (it is not always useful, and
-                   * also it can lead to issues - for instance, if we borrow an
+                   * also it can lead to issues - for instance, if we borrow a
                    * reserved borrow, we later can't translate it to pure values...) *)
                   match rvalue with
                   | E.Global _ -> raise (Failure "Unreachable")
                   | E.Use _
-                  | E.Ref (_, (E.Shared | E.Mut | E.TwoPhaseMut))
+                  | E.Ref (_, (E.Shared | E.Mut | E.TwoPhaseMut | E.Shallow))
                   | E.UnaryOp _ | E.BinaryOp _ | E.Discriminant _
                   | E.Aggregate _ ->
                       let rp = rvalue_get_place rvalue in
