tests/fstar/misc/Loops.Clauses.fst
@@ -19,6 +19,14 @@ unfold
 let sum_with_shared_borrows_decreases (max : u32) (i : u32) (s : u32) : nat =
   if max >= i then max - i else 0
 
+(** [loops::clear]: decreases clause *)
+unfold let clear_decreases (v : vec u32) (i : usize) : nat =
+  if i <= List.Tot.length v then List.Tot.length v - i else 0
+
+(** [loops::list_mem]: decreases clause *)
+unfold let list_mem_decreases (i : u32) (ls : list_t u32) : list_t u32 =
+  ls
+
 (** [loops::list_nth_mut_loop]: decreases clause *)
 unfold
 let list_nth_mut_loop_decreases (t : Type0) (ls : list_t t) (i : u32) : nat =
@@ -27,6 +35,18 @@ let list_nth_mut_loop_decreases (t : Type0) (ls : list_t t) (i : u32) : nat =
 (** [loops::list_nth_shared_loop]: decreases clause *)
 unfold
 let list_nth_shared_loop_decreases (t : Type0) (ls : list_t t) (i : u32) : list_t t =
+  ls
+
+(** [loops::list_nth_mut_loop_with_id]: decreases clause *)
+unfold
+let list_nth_mut_loop_with_id_decreases (t : Type0) (i : u32) (ls : list_t t) :
+  list_t t =
+  ls
+
+(** [loops::list_nth_shared_loop_with_id]: decreases clause *)
+unfold
+let list_nth_shared_loop_with_id_decreases (t : Type0) (l : list_t t)
+  (i : u32) (ls : list_t t) : list_t t =
   ls
 
 (** [loops::list_nth_mut_loop_pair]: decreases clause *)
